progress on deep declassify for linked lists with Cezar

state/LinkedListIFC.fst
@@ -67,7 +67,9 @@ let rec length (a: Type0) (l: linkedList a) {| c:target_lang a |} : IST nat
          | Cons (h, tlref) -> 
            let tl = !tlref in
             eliminate forall (a:Type) (c:target_lang a) (r:ref a). witnessed (is_low_pred r) ==>
-            c.shallowly_witnessed_is_low (sel h0 r) with (linkedList a) (solve) tlref;
+              c.shallowly_witnessed_is_low (sel h0 r) with (linkedList a) (solve) tlref;
+            eliminate forall (a:Type) (c:target_lang a) (r:ref a). witnessed (contains_pred r) ==>
+              c.shallowly_witnessed_contains (sel h0 r) with (linkedList a) (solve) tlref;
             1 + length a tl #c
 
 // examples
@@ -92,4 +94,71 @@ let cycle_length3 () : ST (linkedList nat) (requires fun _ -> True) (ensures fun
     write x (Cons(2, z));
     Cons (2, z)
 
-//TODO: adapt declassify for cycles
+
+// TODO: clean up
+let rec deep_declassify (l: linkedList int) : ST unit 
+  (requires fun h -> shallowly_witnessed_contains l /\ inv_contains_points_to_contains h)
+  (ensures fun h0 x h1 -> (inv_contains_points_to_contains h1) /\
+                           modifies Set.empty h0 h1 /\
+                           shallowly_witnessed_is_low l /\
+                           (forall (a:Type) (c:target_lang a) (r:ref a). 
+                           (h0 `contains` r /\ label_of r h0 <> Low /\ label_of r h1 == Low) ==> c.shallowly_witnessed_is_low (sel h1 r) )
+                           ) =
+  let h0 = get() in
+  match l with 
+  | Nil -> ()
+  | Cons (h, tlref) ->
+    let tl = !tlref in 
+      declassify tlref Low;
+      gst_witness (is_low_pred tlref);
+      eliminate forall (a:Type) (c:target_lang a) (r:ref a). witnessed (contains_pred r) ==>
+        c.shallowly_witnessed_contains (sel h0 r) with (linkedList int) (solve) tlref;
+      let h1 = get () in
+      deep_declassify tl;
+      let h2 = get () in
+      assert ((forall (a:Type) (c:target_lang a) (r:ref a). h0 `contains` r <==> h1 `contains` r));
+      assert ((forall (a:Type) (c:target_lang a) (r:ref a). 
+                (h1 `contains` r /\ label_of r h1 <> Low /\ label_of r h2 == Low) ==> 
+                  c.shallowly_witnessed_is_low (sel h2 r) ));
+
+
+      assert (modifies_classification (only tlref) h0 h1);
+      assert (modifies Set.empty h0 h2);
+      assert (sel h0 tlref == sel h2 tlref);
+      assert (shallowly_witnessed_is_low (sel h2 tlref));
+      assert ((label_of tlref h0 <> Low /\ label_of tlref h2 == Low) ==> 
+                shallowly_witnessed_is_low (sel h2 tlref) );   
+    
+      introduce forall (a:Type) (c:target_lang a) (r:ref a). 
+               (h0 `contains` r /\ label_of r h0 <> Low /\ label_of r h2 == Low) ==> 
+                c.shallowly_witnessed_is_low (sel h2 r)
+      with begin
+        introduce (h0 `contains` r /\ label_of r h0 <> Low /\ label_of r h2 == Low) ==> 
+                c.shallowly_witnessed_is_low (sel h2 r)
+        with _. begin
+          introduce label_of r h1 <> Low ==> c.shallowly_witnessed_is_low (sel h2 r) with _. ();
+          introduce label_of r h1 == Low ==> c.shallowly_witnessed_is_low (sel h2 r) with _. begin
+            assert (addr_of r = addr_of tlref);
+            assume (is_mm r == is_mm tlref);
+            lemma_sel_same_addr' h2 r tlref;
+            assert (shallowly_witnessed_is_low (sel h2 tlref));
+            assert (sel h2 tlref == sel h2 r);
+            // let r : ref (linkedList int) = r in
+            let c : target_lang (linkedList int) = c in
+            assert ((target_lang_linkedList int).shallowly_witnessed_is_low (sel h2 tlref));
+            assume ((forall (a:Type) (c:target_lang a) (c':target_lang a) (v:a) . 
+              c.shallowly_witnessed_is_low v ==> c'.shallowly_witnessed_is_low v));
+            assert (c.shallowly_witnessed_is_low (sel h2 tlref));
+            assert (c.shallowly_witnessed_is_low (sel h2 r));
+            ()
+          end
+        end 
+      end;
+      assert ((forall (a:Type) (c:target_lang a) (r:ref a). 
+          (h0 `contains` r /\ label_of r h0 <> Low /\ label_of r h2 == Low) ==> 
+          c.shallowly_witnessed_is_low (sel h2 r) ));
+      ()
+
+  // let test (l: linkedList int) : IST unit (ensures fun _ -> True) (requires fun _ _ _ -> True) =
+  //   deep_declassify l;
+  //   ()
